More structure added. We need not flush in irreducible nodes. But it would be easier to translate TSO to an equivalent intermediate language that does not have the flush rule

Bisimulation.v
@@ -7,18 +7,19 @@ Require Import Util.
 Require Import Translation.
 
 
-Inductive related : (term * bool) -> (term * bool) -> Prop :=
-  | related_translate : forall e thread base buf_size, related (e, thread) (translate e thread base buf_size, thread).
+Inductive related (base : nat) (buf_size : nat) : (term * bool) -> (term * bool) -> Prop :=
+  | related_translate : forall e thread, related base buf_size (e, thread) (translate e thread base buf_size, thread).
  
 
 Definition related_terms (TSO_program : TSO.program) (SC_program : SC.program) (base : nat) : Prop :=
   let TSO1 := snd (fst TSO_program) in
   let TSO2 := snd TSO_program in
   let SC1 := snd (fst (fst SC_program)) in
-  let SC2 := snd (fst SC_program) in
+  let SC2 := snd (fst SC_program)in
   let SC3 := snd SC_program in
-  related (TSO1, true) (SC1, true) /\
-  related (TSO2, false) (SC2, false) /\
+  let buf_size := fst (fst (fst TSO_program)) in
+  related base buf_size (TSO1, true) (SC1, true) /\
+  related base buf_size (TSO2, false) (SC2, false) /\
   SC3 = while tru ((SPECIAL base) ::= ZERO).
 
 Definition related_memory (TSO_memory : TSO.memory_model) (SC_memory : SC.memory_model) (B : nat) (f : nat -> nat) : Prop :=
@@ -81,14 +82,28 @@ Definition related_program (p : TSO_machine) (q : SC_machine) (f : nat -> nat) (
   related_terms TSO_program SC_program B /\
   related_memory TSO_memory SC_memory B f.
 
-Fact contexts_respect_bisimilarity : forall E B s2 buffer f true e event e' mem mem' m t0 l t1,
-  related (s2, false) (t0, false) ->
+Fact psteps_app : forall t t' x e,
+  SC_program_steps t t' ->
+  SC_program_steps (fst (fst (fst (fst t))), app (lam x e) (snd (fst (fst (fst t)))), snd (fst (fst t)), snd (fst t), snd t) (fst (fst (fst (fst t'))), app (lam x e) (snd (fst (fst (fst t')))), snd (fst (fst t')), snd (fst t'), snd t').
+Proof. intros. induction H.
+  + apply SC_program_steps_reflexive.
+  + destruct q. destruct p. destruct p. destruct p. destruct p. destruct r. destruct p. destruct p. destruct p. destruct p0. destruct p. destruct p. simpl in *. apply SC_program_steps_transitive with (q:=(l1, app (lam x e) t7, t6, t5, m)). inversion H; subst.
+    ++ apply ST_init_allocate_array. auto. auto. auto.
+    ++ apply ST_synchronize1 with (event:=event).
+       assert (exists y e', lam x e = lam y e'). refine (ex_intro _ x _). refine (ex_intro _ e _). reflexivity. assert (app (lam x e) t1 = con_subst (Capp2 (exist _ (lam x e) H1) Hole) t1). simpl. reflexivity. assert (app (lam x e) t7 = con_subst (Capp2 (exist _ (lam x e) H1) Hole) t7). simpl. reflexivity. rewrite H2. rewrite H4. apply step_context. auto. auto.
+    ++ apply ST_synchronize2 with (event:=event). auto. auto.
+    ++ apply ST_synchronize3 with (event:=event). auto. auto.
+    ++ auto.
+Qed.
+
+Fact contexts_respect_bisimilarity : forall E B s2 buffer f e event e' mem mem' m t0 l t1,
+  related B buffer (s2, false) (t0, false) ->
   related_memory mem m B f ->
   step e event e' ->
   TSO.memstep mem (true, event) mem' ->
-  related (con_subst E e, true) (t1, true) ->
+  related B buffer (con_subst E e, true) (t1, true) ->
   (forall re : term,
-  related (e, true) (re, true) ->
+  related B buffer (e, true) (re, true) ->
   exists q' : SC_machine,
   related_program (buffer, nil, e', s2, mem') q' f B /\
   SC_program_steps (l, re, t0, while tru (SPECIAL B [num 0]::= ZERO), m) q') ->
@@ -104,17 +119,28 @@ Proof. intros. generalize dependent t1. induction E; intros; simpl in *.
           SC_program_steps
             (l, translate (con_subst E e) true B buffer, t0,
             while tru (SPECIAL B [num 0]::= ZERO), m)
-            q'). apply IHE. apply related_translate. destruct H5. destruct H5. destruct x. destruct p. destruct p. destruct p. destruct H5. simpl in *. destruct H7. destruct H7. simpl in *. inversion H3. inversion H7. subst. refine (ex_intro _ (l0, translate (app (con_subst E e') t) true B buffer, t3, t2, m0) _). split.
-    ++ unfold related_program. simpl. split.
-      +++ intros. contradiction H10. auto.
+            q'). apply IHE. apply related_translate. destruct H5. destruct H5. destruct x. destruct p. destruct p. destruct p. destruct H5. simpl in *. unfold related_terms in H7. destruct H7. destruct H7. simpl in *. inversion H3. inversion H7. subst. refine (ex_intro _ (l0, translate (app (con_subst E e') t) true B buffer, t3, t2, m0) _). split.
+    ++ split.
+      +++ simpl. intros. contradiction H10. auto.
       +++ split.
         ++++ unfold related_terms. simpl in *. split.
-          - admit.
-          - split.
-            -- admit.
-            -- admit.
-        ++++ admit.
-    ++ simpl. admit.
+          - assert ((translate (app (con_subst E e') t) true B buffer, true) =
+(app (lam "x" (flush_star true B buffer;; var "x")) (app (translate (con_subst E e') true B buffer) (translate t true B buffer)), true)). auto. rewrite <- H10. apply related_translate.
+          - auto.
+        ++++ auto.
+    ++ simpl. remember (l,
+      (app (translate (con_subst E e) true B buffer)
+         (translate t true B buffer)), t0,
+    WHILE tru DO SPECIAL B [num 0]::= ZERO DONE, m) as P1. remember (l0,
+      (app (translate (con_subst E e') true B buffer)
+         (translate t true B buffer)), t3, t2, m0) as P2. assert ((l,
+    app (lam "x" (flush_star true B buffer;; var "x"))
+      (app (translate (con_subst E e) true B buffer)
+         (translate t true B buffer)), t0,
+    WHILE tru DO SPECIAL B [num 0]::= ZERO DONE, m) = (fst (fst (fst (fst P1))), app (lam "x" (flush_star true B buffer;; var "x")) (snd (fst (fst (fst P1)))), snd (fst (fst P1)), snd (fst P1), snd P1)). subst. simpl. auto. rewrite H10. assert ((l0,
+    app (lam "x" (flush_star true B buffer;; var "x"))
+      (app (translate (con_subst E e') true B buffer)
+         (translate t true B buffer)), t3, t2, m0) = (fst (fst (fst (fst P2))), app (lam "x" (flush_star true B buffer;; var "x")) (snd (fst (fst (fst P2)))), snd (fst (fst P2)), snd (fst P2), snd P2)). subst. simpl. auto. rewrite H11. clear H10. clear H11. apply psteps_app. subst. simpl in *. admit.
   + admit.
   + admit.
   + admit.
